\documentclass[letterpaper]{article}
\usepackage{enumerate}
\usepackage{amsmath}
\begin{document}
\begin{equation}
\begin{aligned}
f_{t}&=\sigma(W_{f}x_{t}+U_{f}h_{t-1}+b_{f})\\
i_{t}&=\sigma(W_{i}x_{t}+U_{i}h_{t-1}+b_{i})\\
o_{t}&=\sigma(W_{o}x_{t}+U_{o}h_{t-1}+b_{o})\\
c'_{t}&=\tanh(W_{c}x_{t}+U_{c}h_{t-1}+b_{c})\\
c_{t}&=f_{t}\circ c_{t-1}+i_{t}\circ c'_t\\
h_{t}&=o_{t}\circ \tanh(c_{t})
\end{aligned}
\end{equation}
Variables:\\
$M$: input vector dimension\\
$N$: output vector dimension\\
($H_i$: hidden layer $i$ vector dimension)\\
$x_{t}$ $[M\times 1]$: input vector\\
$h_{t}$ $[N\times 1]$: output vector\\
$h_{0} = 0$\\
$c_{t}$ $[N\times 1]$: cell state vector\\
$c_{0} = 0$\\
$W$ $[N\times M]$, $U$ $[N\times N]$ and $b$ $[N\times 1]$: parameter matrices and vector (W is for weight, U is for update?, and b is for bias?)\\
$f_{t}$, $i_{t}$ and $o_{t}$: gate vectors\\
$f_{t}$ $[N\times 1]$: Forget gate vector. Weight of remembering old information.\\
$i_{t}$ $[N\times 1]$: Input gate vector. Weight of acquiring new information.\\
$o_{t}$ $[N\times 1]$: Output gate vector. Output candidate.

\begin{equation}
\begin{aligned}
\delta h_t +&= target_t - h_t\\
\delta o_t &= \delta h_t \circ \tanh (c_t)\\
\delta c_t +&= \delta h_t \circ o_t \circ \tanh' (c_t)\\
\delta i_t &= \delta c_t \circ c'_t\\
\delta f_t &= \delta c_t \circ c_{t-1}\\
\delta c'_t &= \delta c_t \circ i_t\\
\delta c_{t-1} &= \delta c_t \circ f_t\\
\delta \hat{i}_t &= \delta c_t \circ c'_t\\
\delta \hat{f}_t &= \delta c_t \circ c_{t-1}\\
\delta \hat{c'}_t &= \delta c'_t \circ (1 - c'^2_t)\\
\delta \hat{i}_t &= \delta i_t \circ i_t \circ (1-i_t)\\
\delta \hat{f}_t &= \delta f_t \circ f_t \circ (1-f_t)\\
\delta \hat{o}_t &= \delta o_t \circ o_t \circ (1-o_t)\\
\delta W_{i,f,o,c} &= \delta {\hat{i},\hat{f},\hat{o},\hat{c'}}_t x^T_t\\
\delta U_{i,f,o,c} &= \delta {\hat{i},\hat{f},\hat{o},\hat{c'}}_t h^T_{t-1}\\
\delta b_{i,f,o,c} &= \delta {\hat{i},\hat{f},\hat{o},\hat{c'}}_t\\
\delta h_{t-1} &= \sum U_{i,f,o,c}^T\delta {\hat{i},\hat{f},\hat{o},\hat{c'}}_t\\
\end{aligned}
\end{equation}
$\delta h_{T} = 0$\\
$\delta c_{T} = 0$\\

\begin{equation}
\begin{aligned}
\delta y_t &= \Delta_t + R_z\delta z_{t+1} + R_i\delta i_{t+1} + R_f\delta f_{t+1} + R_o\delta o_{t+1}\\
\delta x_t &= W_z\delta z_{t} + W_i\delta z_{t} + W_f\delta f_{t} + W_o\delta o_{t}\\
\delta W_{\star} &= \sum^T_{t=0} \langle \delta\star_t,x_t\rangle\\
\delta R_{\star} &= \sum^{T-1}_{t=0} \langle \delta\star_{t+1},y_t\rangle\\
\delta b_{\star} &= \sum^{T}_{t=0} \delta\star_{t}\\
\delta p_{i} &= \sum^{T-1}_{t=0} c_t \circ \delta i_{t+1}\\
\delta p_{f} &= \sum^{T-1}_{t=0} c_t \circ \delta f_{t+1}\\
\delta p_{o} &= \sum^{T}_{t=0} c_t \circ \delta o_{t}\\
\end{aligned}
\end{equation}

\end{document}